

$$
{\phi \vdash \psi }\\
{\underline {\phi \vdash \lnot \psi}}\\
{\lnot \phi}
$$

---

$$
\begin{array}{lll}
1 & R &Premise 1 \\
2 & S &Premise 2 \\
\hline
. & . &.\\
. & . &.\\
. & . &.\\
\hline
n & Conclusion & Justification \\
\end{array}
$$

---

$$
\begin{align}
(a+b)^2 &= (a+b)(a+b)          \tag{3.1c}      \\
        &= a^2 + ab + ba + b^2 \tag{$\dagger$} \\
        &= a^2 + 2ab + b^2     \tag{$\ast$}
\end{align}
$$

---

$$
\begin{align}
\text{To prove it by contradiction try and assume that the statemenet is false,
proceed from there and at some point you will arrive to a contradiction.}
\end{align}
$$
